Hs/Metatheory/Preservation.lean
@@ -38,6 +38,23 @@ inductive HsTypeLike : Ctx HsTerm -> HsTerm -> Term -> Prop
 | HsAll : HsTypeLike (.kind A :: Γ) t t' -> HsKindLike A A' -> HsTypeLike Γ (`∀{A} t) (∀[A']t')
 | HsAppk : HsTypeLike Γ t1 t1' -> HsTypeLike Γ t2 t2' -> HsTypeLike Γ (t1 `•k t2) (t1' `@k t2')
 
+theorem weaken_term_hs_type_like :
+  HsTypeLike Γ τ τ' ->
+  Γ ⊢s t : A ->
+  HsTypeLike (.term A t :: Γ) ([S]τ) ([S]τ') := by sorry
+
+theorem hs_type_like_unique :
+  HsTypeLike Γ τ τ' -> HsTypeLike Γ τ τ'' -> τ' = τ'' := by
+intro j1 j2;
+induction j2;
+case _ h1 h2 ih1 ih2 =>
+  -- have lem1 :=  ih1 h1;
+  -- have lem2 :=  ih2 h2;
+  sorry
+case _ => sorry
+case _ => sorry
+case _ => sorry
+
 @[simp]
 abbrev  CompilePreservesTypes : (v : CompileVariant) -> (Γ : Ctx HsTerm) -> CompileJArgs v Γ -> Prop
 | .type => λ Γ => λ ⟨τ, k; j, τ'⟩ =>
@@ -73,6 +90,17 @@ intro j1 j2;
 have lem := compile_preserves_type_shape_lemma j2; simp at lem;
 apply lem j2;
 
+theorem compile_type_uniqueness :
+  (j : Γ ⊢s A : `★) ->
+  CompileJ .type Γ ⟨A, `★; j, A'⟩ ->
+  CompileJ .type Γ ⟨A, `★; j, A''⟩ ->
+  A' = A''
+:= by
+intro j1 c1 c2;
+have lem1 := compile_preserves_type_shape j1 c1;
+have lem2 := compile_preserves_type_shape j1 c2;
+apply hs_type_like_unique lem1 lem2;
+
 
 theorem compile_preserves_indices :
   CompileJ .ctx Γ Γ' ->
@@ -80,7 +108,21 @@ theorem compile_preserves_indices :
   CompileJ .type Γ ⟨τ, `★; j, τ'⟩ ->
   (Γ' d@ x).get_type = .some τ' := by
 intro cc gt cτ;
-induction x <;> simp at *; simp at j;
+cases cc;
+case _ => cases gt
+case _ =>
+  simp at j;
+  induction x;
+  case _ => cases gt
+  case _ n ih =>
+  simp at gt;
+  cases gt; case _ w gt =>
+  cases gt; case _ gt e =>
+  subst e;
+  sorry
+case _ => sorry
+case _ => sorry
+case _ => sorry
 case _ => sorry
 case _ => sorry
 
@@ -177,7 +219,7 @@ case _ Γ _ _  A' _ Γ' j1 j2 c1 c2 c3 ih1 ih2 ih3 =>
   have ih1'' := ih1' cc .HsType (HsJudgment.ax wf) (CompileJ.type _) c1; assumption
   have ih2' := ih2 Γ' A' c3 (compile_preserves_type_shape j1' c1') c2 j1 c1; assumption;
   apply ih3 wf c3
-case _ wf =>
+case type =>
   intro Γ' cc cc'
   cases cc';
   apply Judgment.ax;
@@ -235,6 +277,10 @@ case appev Γ π τ e t1 π' τ' e' t1' τ'' j1 j2 j3 j4 _ c1 c2 c3 c4 eq c5 ih1
 
 case appt => sorry
 
+case lamt => sorry
+
+case lamev => sorry
+
 case var Γ x τ wf gt j1 =>
   intro Γ' τ' cc tl cc' jτ cτ
   have lem := compile_preserves_indices cc gt cτ;
@@ -243,20 +289,40 @@ case var Γ x τ wf gt j1 =>
 case app j1 j2 j3 c1 c2 ih1 ih2 => sorry
 
 case lam Γ A t1 τ A' t1' j1 j2 j3 c1 c2 ih1 ih2 =>
-  intro Γ' τ' cc c1' jk ck cτ;
-  cases c1'; case _ τ1' τ2' tl1 tl2 =>
-  have ih1' := ih1 Γ' ★ cc .HsType (HsJudgment.ax (hs_judgment_ctx_wf .prf j1)) sorry c1;
-  have ih2' := ih2 (.type A' :: Γ') τ2' sorry sorry c2
+  intro Γ' τ' cc tl cc' jτ cτ;
+  cases tl; case _ τ1' τ2' tl1 tl2 =>
+  cases cτ; case _  j1' j1' j2' c2' =>
+  have lem1 := compile_preserves_type_shape j1 c1;
+  have e := hs_type_like_unique tl1 lem1; symm at e; subst e;
+  have lem2 := compile_preserves_type_shape j1' c2';
+  apply Judgment.lam;
+  apply ih1 Γ' ★ cc .HsType (HsJudgment.ax (hs_judgment_ctx_wf .prf j1)) (CompileJ.type _) c1;
+  have ih2' := ih2 (.empty ::Γ') τ2' sorry
+  sorry
   sorry
 
+  -- cases c1'; case _ τ1' τ2' tl1 tl2 =>
+  -- have ih1' := ih1 Γ' ★ cc .HsType (HsJudgment.ax (hs_judgment_ctx_wf .prf j1)) sorry c1;
+  -- have ih2' := ih2 (.type A' :: Γ') τ2' sorry sorry c2
+  -- have lem := @Judgment.lam Γ' A' t1' τ2' ih1' sorry sorry;
+  -- sorry
 
-case _ =>
-  intro Γ' τ' cc tl c4 j1 c1
+case _ Γ A τ t1 t2 A' τ' t1' t2' j1 j2 j3 j4 j5 c1 c2 c3 c4 ih1 ih2 ih3 ih4 =>
+  intro Γ' τ'' cc tl cc' j1' c1'
   apply Judgment.letterm
-  sorry
-  sorry
-  sorry
-  sorry
+  apply ih1 Γ' ★ cc .HsType (HsJudgment.ax (hs_judgment_ctx_wf .prf j1)) (CompileJ.type _) c1
+  clear ih1;
+  apply ih3 Γ' A' cc (compile_preserves_type_shape j1 c1) c3 j1 c1
+  clear ih3;
+  have lem1 := CompileJ.wfterm j1 j3 c1 c3 cc;
+  have lem2 := weaken_term_hs_type_like tl j3
+  have lem3 := hs_weaken_term j1 j3 j2;
+  apply ih4 (.term A' t1':: Γ') ([S]τ'') _ _ c4 lem3 _
+  case _ => apply lem1
+  case _ => apply lem2
+  case _ => sorry
+  sorry -- apply ih2 Γ' ★ cc sorry c2 j1 c1;
+
 case _ =>
   intro Γ' τ' cc tl c5 j1 c1
   apply Judgment.ite;
@@ -273,47 +339,3 @@ case _ =>
   sorry
   sorry
   sorry
-
-
--- @[simp]
--- abbrev CompileTypePreservingType : (v : CompileVariant) -> (Γ : Ctx HsTerm) -> CompileJArgs v Γ -> Prop
--- | .term => λ Γ => λ ⟨t, τ ; j, t'⟩ => ∀ Γ' τ',
---   ⊢s Γ ->
---   CompileJ .ctx Γ Γ' ->
---   ⊢ Γ' ->
---   (jτ : Γ ⊢s τ : `★) ->
---   CompileJ .term Γ ⟨τ, `★ ; jτ, τ'⟩ ->
---   CompileJ .term Γ ⟨t, τ ; j, t'⟩ ->
---   Γ' ⊢ t' : τ'
--- | .ctx => λ _ => λ _ => true
-
--- theorem compile_type_preserving :
---   CompileJ v Γ idx ->
---   CompileTypePreservingType v Γ idx
---  := by sorry
--- intro j; induction j <;> simp at *;
--- all_goals (intro Γ' τ' wf cc wf' jτ c1 c2)
--- case _ => sorry
--- case _ j1 j2 j3 ck1 ck2 ih1 ih2 => cases c1
--- case _ j1 c1 j2 j3 j4 c2 ih1 ih2 ih3 => -- bogus case
---   sorry
--- case _ =>
---   cases c2; case _ gt =>
---   have h := compile_type_preserving_index cc gt c1;
---   apply Judgment.var wf' (Eq.symm h)
-
--- theorem compile_valid_ctor_preserving :
---   (j : Γ ⊢s A : `★) ->
---   Compile A j A' ->
---   CompileCtx Γ Γ' ->
---   ValidHsCtorType Γ A ->
---   ValidCtorType Γ' A' := by
--- intro j c1 c2 h;
--- induction h;
--- case _ => sorry
--- case _ j' ih =>
---   have lem := compile_kind_preserving1 j
---   replace ih := ih j';
---   sorry
--- case _ => sorry
--- case _ => sorry
